README.md
@@ -1,5 +1,1 @@
 # private-RAG
-
-```
-python path_ORAM/path_ORAM.py in.txt out.txt
-```
